src/high/locations.v
@@ -1,0 +1,666 @@
+(* Assertions for locations.
+
+  The assertions here are modeled usin the more resources defined in
+  [self.high.resources], etc.
+ *)
+
+From iris.bi Require Import lib.fractional.
+From iris.base_logic.lib Require Import own.
+From iris.algebra Require Import gset gmap excl auth.
+From iris.proofmode Require Import reduction monpred tactics.
+From iris_named_props Require Import named_props.
+
+From self Require Import extra ipm_tactics.
+From self.algebra Require Import ghost_map.
+From self.lang Require Import lang.
+From self.base Require Import primitive_laws.
+From self.high Require Import dprop abstract_state lifted_modalities or_lost.
+From self.high Require Export abstract_state resources protocol modalities post_crash_modality.
+From self.high.resources Require Export bumpers preorders auth_map_map abstract_history.
+From self.high.modalities Require Export no_buffer.
+
+Definition increasing_list `{SqSubsetEq ST} (ss : list ST) :=
+  ∀ i j s s', i < j → (ss !! i = Some s) → (ss !! j = Some s') → s ⊑ s'.
+
+Lemma increasing_list_singleton `{SqSubsetEq ST} (s : ST) : increasing_list [s].
+Proof. intros [|][|]?????; try naive_solver. simplify_eq. lia. Qed.
+
+Lemma lookup_snoc_Some {A} (l : list A) x x2 i :
+  (l ++ [x]) !! i = Some x2 →
+  (l !! i = Some x2) ∨ (length l = i ∧ x = x2).
+Proof.
+  intros [look|[? [??]%list_lookup_singleton_Some]]%lookup_app_Some.
+  - left. apply look.
+  - right. auto with lia.
+Qed.
+
+Lemma increasing_list_snoc `{SqSubsetEq ST} xs xs__last (x : ST) :
+  (last xs) = Some xs__last →
+  xs__last ⊑ x →
+  increasing_list xs → increasing_list (xs ++ [x]).
+Proof.
+  intros last incl incr.
+  intros ?????.
+  intros [?|[??]]%lookup_snoc_Some; intros [look|[??]]%lookup_snoc_Some.
+  * eapply incr; done.
+  * simplify_eq.
+    admit.
+  * apply lookup_lt_Some in look. lia.
+  * lia.
+Admitted.
+
+Section points_to_at.
+  Context `{nvmFixedG Σ, hGD : nvmDeltaG Σ, AbstractState ST}.
+
+  Implicit Types (ℓ : loc) (s : ST) (ss : list ST) (prot : LocationProtocol ST).
+
+  Definition abs_hist_to_ra_old
+          (abs_hist : gmap time (message * positive)) : encoded_abs_historyR :=
+    (to_agree ∘ snd) <$> abs_hist.
+
+  Lemma singleton_included_l' `{Countable K, CmraTotal A}
+        (m : gmap K A) (i : K) x :
+    {[i := x]} ≼ m ↔ (∃ y : A, m !! i ≡ Some y ∧ x ≼ y).
+  Proof.
+    setoid_rewrite <-(Some_included_total x).
+    apply singleton_included_l.
+  Qed.
+
+  (* Points-to predicate for non-atomics. This predcate says that we know that
+the last events at [ℓ] corresponds to the *)
+  Program Definition mapsto_na (ℓ : loc) prot (* (per : bool) *) (q : frac) (ss : list ST) : dProp Σ :=
+    (∃ (tP tStore : time) SV (abs_hist : gmap time ST) (msg : message),
+      "#locationProtocol" ∷ ⎡ know_protocol ℓ prot ⎤ ∗
+      (* NOTE: Maybe we can actually remove [increasing_list]? It should be
+      covered by the fact that the list corresponds to [abs_hist] and that one
+      is sorted. *)
+      "%incrList" ∷ ⌜ increasing_list ss⌝ ∗
+      "#isNaLoc" ∷ ⎡ is_na_loc ℓ ⎤ ∗
+
+      (* [tStore] is the last message and it agrees with the last state in ss. *)
+      "%lookupV" ∷ ⌜ abs_hist !! tStore = last ss ⌝ ∗
+      "%nolater" ∷ ⌜ map_no_later abs_hist tStore ⌝ ∗
+
+      (* Ownership over the full abstract history. *)
+      "hist" ∷ ⎡ know_full_history_loc ℓ q abs_hist ⎤ ∗
+
+      "knowSV" ∷ ⎡ know_na_view ℓ q SV ⎤ ∗
+      "%slice" ∷ ⌜ map_slice abs_hist tP tStore ss ⌝ ∗
+      "#physMsg" ∷ ⎡ auth_map_map_frag_singleton know_phys_history_name ℓ tStore msg ⎤ ∗
+      (* "%msgViewIncluded" ∷ ⌜ msg_store_view msg ⊑ SV ⌝ ∗ *)
+      "#inThreadView" ∷ monPred_in (SV, msg_persisted_after_view msg, ∅) ∗
+      (* We have the [tStore] timestamp in our store view. *)
+      "%haveTStore" ∷ ⌜ tStore ≤ SV !!0 ℓ ⌝ ∗
+      (* "haveTStore" ∷ monPred_in ({[ ℓ := MaxNat tStore ]}, ∅, ∅) ∗ *)
+
+      "#pers" ∷ (⎡ persisted_loc ℓ tP ⎤ ∨ ⌜ tP = 0 ⌝)
+    )%I.
+
+  Global Instance mapsto_na_fractional ℓ prot ss :
+    Fractional (λ q, mapsto_na ℓ prot q ss).
+  Proof.
+    intros p q.
+    rewrite /mapsto_na.
+    iSplit.
+    - iNamed 1.
+      iDestruct "hist" as "[histP histQ]".
+      iDestruct "knowSV" as "[knowSVP knowSVQ]".
+        iSplitL "histP knowSVP".
+        + iExists _, _, _, _, _.
+          iFrame "#∗%".
+        + iExists _, _, _, _, _.
+          iFrame "#∗%".
+      (* destruct per. *)
+      (* * iDestruct "pers" as "#pers". *)
+      (*   iSplitL "histP knowSVP". *)
+      (*   + iExists _, _, _, _, _. *)
+      (*     iFrame "#∗%". *)
+      (*   + iExists _, _, _, _, _. *)
+      (*     iFrame "#∗%". *)
+      (* * iDestruct "pers" as "#pers". *)
+      (*   iSplitL "histP knowSVP". *)
+      (*   + iExists _, _, _, _, _. *)
+      (*     iFrame "#∗%". *)
+      (*   + iExists _, _, _, _, _. *)
+      (*     iFrame "#∗%". *)
+    - iDestruct 1 as "[L R]".
+      iNamed "L".
+      iDestruct "R" as (?????) "(_ & _ & _ & _ & _ & histQ & SV & HIP & ?)".
+      iDestruct (ghost_map_elem_agree with "hist histQ") as %->%(inj (fmap _)).
+      iDestruct (ghost_map_elem_agree with "knowSV SV") as %->.
+      iExists _, _, _, _, _. iFrame "#∗%".
+  Qed.
+  Global Instance mapsto_na_as_fractional ℓ prot q v :
+    AsFractional (mapsto_na ℓ prot q v) (λ q, mapsto_na ℓ prot q v)%I q.
+  Proof. split; [done | apply _]. Qed.
+
+  Program Definition have_SV ℓ t : dProp Σ :=
+    MonPred (λ TV, ⌜ t ≤ (store_view TV) !!0 ℓ ⌝)%I _.
+  Next Obligation. solve_proper. Qed.
+
+  Global Instance have_SV_persistent ℓ t : Persistent (have_SV ℓ t).
+  Proof. apply monPred_persistent=> j. apply _. Qed.
+
+  Program Definition have_FV ℓ t : dProp Σ :=
+    MonPred (λ TV, ⌜ t ≤ (flush_view TV) !!0 ℓ ⌝)%I _.
+  Next Obligation. solve_proper. Qed.
+
+  Global Instance have_FV_persistent ℓ t : Persistent (have_FV ℓ t).
+  Proof. apply monPred_persistent=> j. apply _. Qed.
+
+  Lemma have_SV_0 ℓ : ⊢ have_SV ℓ 0.
+  Proof. iModel. iPureIntro. lia. Qed.
+
+  Lemma have_FV_0 ℓ : ⊢ have_FV ℓ 0.
+  Proof. iModel. iPureIntro. lia. Qed.
+
+  Definition know_store_lb ℓ prot (s : ST) : dProp Σ :=
+    ∃ (tS : nat),
+      "#locationProtocol" ∷ ⎡ know_protocol ℓ prot ⎤ ∗
+      "#knowFragHist" ∷ ⎡ know_frag_history_loc ℓ {[ tS := s ]} ⎤ ∗
+      "#tSLe" ∷ have_SV ℓ tS.
+
+  (* Program Definition know_store_lb ℓ prot (s : ST) : dProp Σ := *)
+  (*   MonPred (λ TV, *)
+  (*     ∃ (tS : nat) (* (msg : message) *), *)
+  (*       "#locationProtocol" ∷ know_protocol ℓ prot ∗ *)
+  (*       "#knowFragHist" ∷ know_frag_history_loc ℓ {[ tS := s ]} ∗ *)
+  (*       "%tSLe" ∷ ⌜ tS ≤ (store_view TV) !!0 ℓ ⌝ *)
+  (*   )%I _. *)
+  (* Next Obligation. solve_proper. Qed. *)
+
+  Definition know_flush_lb ℓ prot (s : ST) : dProp Σ :=
+    ∃ (tF : nat),
+      "#locationProtocol" ∷ ⎡ know_protocol ℓ prot ⎤ ∗
+      "knowFragHist" ∷ ⎡ know_frag_history_loc ℓ {[ tF := s ]} ⎤ ∗
+      (* "%tSLe" ∷ ⌜ tF ≤ (store_view TV) !!0 ℓ ⌝ ∗ *)
+      "#tSLe" ∷ have_SV ℓ tF ∗
+      (* Either the location is persisted or we have something in the flush
+      view. The later case is for use after a crash where we don't have
+      anything in the flush view. *)
+      (* Note: I think the below should be changed to: (∃ t, flush_view TV !!
+        ℓ = Some t ∧ tF ≤ t ∨ persisted_loc ℓ tF) Otherwise we wouldn't be
+        able to show the [wp_wb] rule for a freshly allocated location with a
+        message at 0. *)
+      "viewFact" ∷ (⌜tF ≠ 0⌝ ∗ have_FV ℓ tF ∨
+                    ⌜tF = 0⌝ ∗ ⎡ persisted_loc ℓ 0 ⎤ )%I.
+  (* Next Obligation. solve_proper. Qed. *)
+
+  Program Definition know_persist_lb ℓ prot (sP : ST) : dProp Σ :=
+    ∃ tP,
+      "#locationProtocol" ∷ ⎡ know_protocol ℓ prot ⎤ ∗
+      "knowFragHist" ∷ ⎡ know_frag_history_loc ℓ {[ tP := sP ]} ⎤ ∗
+      (* We have the persisted state in our store view. *)
+      "#tSLe" ∷ have_SV ℓ tP ∗
+      "#tPLe" ∷ have_FV ℓ tP ∗
+      "persisted" ∷ ⎡ persisted_loc ℓ tP ⎤.
+
+  (* Program Definition know_persist_lb ℓ prot (sP : ST) : dProp Σ := *)
+  (*   MonPred (λ TV, *)
+  (*     ∃ tP, *)
+  (*       "#locationProtocol" ∷ know_protocol ℓ prot ∗ *)
+  (*       "knowFragHist" ∷ know_frag_history_loc ℓ {[ tP := sP ]} ∗ *)
+  (*       (* We have the persisted state in our store view. *) *)
+  (*       "%tSLe" ∷ ⌜ tP ≤ (store_view TV) !!0 ℓ ⌝ ∗ *)
+  (*       "%tPLe" ∷ ⌜ tP ≤ (flush_view TV) !!0 ℓ ⌝ ∗ *)
+  (*       "persisted" ∷ persisted_loc ℓ tP *)
+  (*   )%I _. *)
+  (* Next Obligation. solve_proper. Qed. *)
+
+  (* The location [ℓ] was recovered in the abstract state [s]. *)
+  Definition recovered_at ℓ s : dProp Σ :=
+    ∃ CV,
+      "#knowFragHist" ∷ ⎡know_frag_history_loc ℓ {[ 0 := s ]}⎤ ∗
+      "#crashed" ∷ ⎡ crashed_at CV⎤ ∗
+      "%inCV" ∷ ⌜ℓ ∈ dom (gset _) CV⌝.
+
+  (* [ℓ] was recovered at the last crash. *)
+  Definition recovered ℓ : dProp Σ := ∃ s, recovered_at ℓ s.
+
+  (* [ℓ] was not recovered at the last crash. *)
+  Definition lost ℓ : dProp Σ :=
+    ∃ CV,
+      "#crashed" ∷ ⎡crashed_at CV⎤ ∗
+      "%notInCV" ∷ ⌜ℓ ∉ dom (gset _) CV⌝.
+
+  (* Let's see if we want this.
+  Definition mapsto_shared ℓ s1 s2 s3 ϕ : dProp Σ :=
+    "knowPred" ∷ ⎡ know_pred ℓ ϕ ⎤ ∗
+    "isSharedLoc" ∷ ⎡ own shared_locs_name (◯ {[ ℓ ]}) ⎤ ∗
+    "globalPerLB" ∷ know_persist_lb ℓ s1 ∗
+    "persistLB" ∷ know_flush_lb ℓ s2 ∗
+    "storeLB" ∷ know_store_lb ℓ s3.
+  *)
+
+  Global Instance know_store_lb_persistent
+         ℓ prot (s : ST) : Persistent (know_store_lb ℓ prot s).
+  Proof. apply _. Qed.
+
+  Global Instance know_flush_lb_persistent
+         ℓ prot (s : ST) : Persistent (know_flush_lb ℓ prot s).
+  Proof. apply _. Qed.
+
+  Global Instance know_persist_lb_persistent
+         ℓ prot (s : ST) : Persistent (know_persist_lb ℓ prot s).
+  Proof. apply _. Qed.
+
+  Lemma persist_lb_to_flush_lb ℓ prot s :
+    know_persist_lb ℓ prot s -∗ know_flush_lb ℓ prot s.
+  Proof.
+    iNamed 1. iExists _. iFrame "∗#".
+    destruct (decide (tP = 0)) as [->|neq].
+    - iRight. iFrame. done.
+    - iLeft. done.
+  Qed.
+
+  Lemma flush_lb_to_store_lb ℓ prot s :
+    know_flush_lb ℓ prot s -∗ know_store_lb ℓ prot s.
+  Proof. iNamed 1. iExists _. iFrame "∗#". Qed.
+
+  Lemma persist_lb_to_store_lb ℓ prot s :
+    know_persist_lb ℓ prot s -∗ know_store_lb ℓ prot s.
+  Proof. iNamed 1. iExists _. iFrame "∗#". Qed.
+  
+  (* Lemma know_flush_lb_at_zero ℓ (s s' : ST) : *)
+  (*   s ⊑ s' → *)
+  (*   ⎡ know_frag_history_loc ℓ {[0 := s']} ⎤ -∗ *)
+  (*   ⎡ know_preorder_loc ℓ abs_state_relation ⎤ -∗ *)
+  (*   know_flush_lb ℓ s. *)
+  (* Proof. *)
+  (*   iStartProof (iProp _). iIntros (incl ?) "?". *)
+  (*   iIntros (? ?) "?". iExists 0, s'. iFrame "%∗". iPureIntro. lia. *)
+  (* Qed. *)
+
+  (*
+  Lemma know_store_lb_at_zero ℓ (s s' : ST) :
+    s ⊑ s' →
+    ⎡ know_frag_history_loc ℓ {[0 := s']} ⎤ -∗
+    ⎡ know_preorder_loc ℓ abs_state_relation ⎤ -∗
+    know_store_lb ℓ s.
+  Proof.
+    iStartProof (iProp _). iIntros (incl ?) "?".
+    iIntros (? ?) "?". iExists 0, s'. iFrame "%∗". iPureIntro. lia.
+  Qed.
+  *)
+
+  (* A few utility lemmas. *)
+  Lemma recovered_at_not_lot ℓ s : recovered_at ℓ s -∗ lost ℓ -∗ False.
+  Proof.
+    iNamed 1. iIntros "(%CV' & crashed' & %notInCV)".
+    iDestruct (crashed_at_agree with "[$] [$]") as %->.
+    set_solver.
+  Qed.
+
+  Lemma recovered_at_agree ℓ s s' :
+    recovered_at ℓ s -∗ recovered_at ℓ s' -∗ ⌜ s = s' ⌝.
+  Proof. Admitted.
+
+  Lemma mapsto_na_store_lb ℓ prot q ss s :
+    last ss = Some s →
+    mapsto_na ℓ prot q ss -∗
+    know_store_lb ℓ prot s.
+  Proof. Admitted.
+
+  Lemma mapsto_na_last ℓ prot q ss : mapsto_na ℓ prot q ss -∗ ⌜∃ s, last ss = Some s⌝.
+  Proof.
+    rewrite /mapsto_na.
+    iNamed 1.
+    apply map_slice_lookup_hi_alt in slice.
+    naive_solver.
+  Qed.
+
+  Lemma mapsto_na_store_lb_incl ℓ prot q ss s1 s2 :
+    last ss = Some s1 →
+    know_store_lb ℓ prot s2 -∗
+    mapsto_na ℓ prot q ss -∗
+    ⌜s2 ⊑ s1⌝.
+  Proof. Admitted.
+
+  Lemma mapsto_na_flush_lb_incl ℓ prot q ss s1 s2 :
+    last ss = Some s1 →
+    know_flush_lb ℓ prot s2 -∗
+    mapsto_na ℓ prot q ss -∗
+    ⌜s2 ⊑ s1⌝.
+  Proof. Admitted.
+
+  (* Instances. *)
+
+  Lemma no_buffer_know_flush_lb ℓ prot (s : ST) :
+    know_flush_lb ℓ prot s -∗ <nobuf> know_flush_lb ℓ prot s.
+  Proof.
+    rewrite /know_flush_lb.
+    iModel.
+    simpl.
+    iDestruct 1 as (?) "HI". iExists _. iFrame.
+  Qed.
+
+  Global Instance buffer_free_know_flush_lb ℓ prot (s : ST) :
+    BufferFree (know_flush_lb ℓ prot s).
+  Proof. rewrite /IntoNoBuffer. eauto using no_buffer_know_flush_lb. Qed.
+
+  Lemma no_buffer_know_store_lb ℓ prot (s : ST) :
+    know_store_lb ℓ prot s -∗ <nobuf> know_store_lb ℓ prot s.
+  Proof.
+    rewrite /know_store_lb.
+    iModel.
+    simpl.
+    iDestruct 1 as (?) "HI". iExists _. iFrame.
+  Qed.
+
+  Global Instance into_no_buffer_know_store_lb ℓ prot (s : ST) :
+    BufferFree (know_store_lb ℓ prot s).
+  Proof. rewrite /IntoNoBuffer. eauto using no_buffer_know_store_lb. Qed.
+
+  Global Instance mapsto_na_buffer_free ℓ prot q (ss : list ST) :
+    BufferFree (mapsto_na ℓ prot q ss).
+  Proof. rewrite /mapsto_na. apply _. Qed.
+
+End points_to_at.
+
+(** Notation for the exclusive points-to predicate. *)
+Notation "l ↦_{ prot } ss" := (mapsto_na l prot 1 ss) (at level 20).
+Notation "l ↦_{ prot }^{ q } ss" := (mapsto_na l prot q ss) (at level 20).
+(* Notation "l ↦^{ p } ss" := (mapsto_na p l 1 ss) (at level 20). *)
+(* Notation "l ↦ ss" := (mapsto_na false l 1 ss) (at level 20). *)
+(* Notation "l ↦{ q } ss" := (mapsto_na false l q ss) (at level 20). *)
+(* Notation "l ↦ₚ ss" := (mapsto_na true l 1 ss) (at level 20). *)
+(* Notation "l ↦ₚ{ q } ss" := (mapsto_na true l q ss) (at level 20). *)
+(* Notation "l ↦ xs ; ys | P" := (mapsto_na l xs ys P) (at level 20). *)
+
+(** Notation for the shared points-to predicate. *)
+(* Notation "l ↦ ( s1 , s2 , s3 )  | P" := (mapsto_shared l s1 s2 s3 P) (at level 20). *)
+
+Section points_to_at_more.
+  Context `{nvmFixedG Σ, hGD : nvmDeltaG Σ, AbstractState ST}.
+
+  Implicit Types (e : expr) (ℓ : loc) (s : ST)
+           (ss : list ST) (prot : LocationProtocol ST).
+
+  Lemma post_crash_know_persist_lb (ℓ : loc) prot (s : ST) :
+    know_persist_lb ℓ prot s -∗
+    post_crash (λ hG, ∃ s', ⌜s ⊑ s'⌝ ∗
+      know_persist_lb ℓ prot (prot.(bumper) s')).
+  Proof.
+    iNamed 1.
+    rewrite /know_protocol. rewrite 2!embed_sep.
+    iDestruct "locationProtocol" as "(-#pred & -#order & -#bumper)".
+    iDestruct (post_crash_frag_history with "[$bumper $knowFragHist]") as "H".
+    iCrash.
+
+    (* rewrite embed_sep. *)
+    iDestruct "persisted" as "(persisted & (% & % & [% %] & #crashed))".
+    iDestruct (or_lost_with_t_get with "[$] H") as "(% & % & bumper & hist)";
+      first done.
+    iDestruct (or_lost_get with "[$] pred") as "pred"; first done.
+    iDestruct (or_lost_get with "[$] order") as "order"; first done.
+    iExists s'.
+    iSplitPure; first intuition.
+    iExists 0.
+    iFrame "∗#".
+    iDestruct (have_SV_0) as "$".
+    iDestruct (have_FV_0) as "$".
+  Qed.
+
+  Lemma post_crash_know_flush_lb (ℓ : loc) prot (s : ST) :
+    know_flush_lb ℓ prot s -∗
+    post_crash (λ hG,
+                  or_lost ℓ (∃ (s' : ST), know_persist_lb ℓ prot s')).
+  Proof.
+    iNamed 1.
+    rewrite /know_protocol. rewrite 2!embed_sep.
+    iDestruct "locationProtocol" as "(-#pred & -#order & -#bumper)".
+    (* iNamed "locationProtocol". *)
+    iDestruct (post_crash_frag_history with "[$bumper $knowFragHist]") as "H".
+    iCrash.
+    iCombine "pred order H" as "H".
+    rewrite 2!or_lost_with_t_sep.
+    iApply (or_lost_with_t_mono_strong with "[] H").
+    iIntros (??). iNamed 1. iIntros "(pred & order & (% & H & bump & hist))".
+    iExists (bumper prot s').
+    rewrite /know_persist_lb.
+    iExists 0.
+    rewrite /know_protocol. iEval (rewrite 2!embed_sep).
+    iFrame "∗#".
+    iDestruct (have_SV_0) as "$".
+    iDestruct (have_FV_0) as "$".
+  Qed.
+
+  Lemma post_crash_know_store_lb (ℓ : loc) prot (s : ST) :
+    know_store_lb ℓ prot s -∗
+    post_crash (λ hG, or_lost ℓ (∃ (s' : ST),
+      know_persist_lb ℓ prot s')).
+  Proof.
+    iNamed 1.
+    rewrite /know_protocol. rewrite 2!embed_sep.
+    iDestruct "locationProtocol" as "(-#pred & -#order & -#bumper)".
+    (* iNamed "locationProtocol". *)
+    iDestruct (post_crash_frag_history with "[$bumper $knowFragHist]") as "H".
+    iCrash.
+    iCombine "pred order H" as "H".
+    rewrite 2!or_lost_with_t_sep.
+    iApply (or_lost_with_t_mono_strong with "[] H").
+    iIntros (??). iNamed 1. iIntros "(pred & order & (% & H & bump & hist))".
+    iExists (bumper prot s').
+    rewrite /know_persist_lb.
+    iExists 0.
+    rewrite /know_protocol. iEval (rewrite 2!embed_sep).
+    iFrame "∗#".
+    iDestruct (have_SV_0) as "$".
+    iDestruct (have_FV_0) as "$".
+  Qed.
+
+  (* NOTE: This rule should be changed once the "bump-back function" is
+  introduced. *)
+  (* Lemma post_crash_mapsto_persisted_ex ℓ prot q (ss : list ST) : *)
+  (*   ℓ ↦_{prot}^{q} ss -∗ <PC> hG', ∃ s, ⌜s ∈ ss⌝ ∗ ℓ ↦_{prot}^{q} [s] ∗ recovered_at ℓ s. *)
+  (* Proof. *)
+  (*   rewrite /mapsto_na. iNamed 1. *)
+  (*   iDestruct "isNaLoc" as "-#isNaLoc". *)
+    (* iDestruct "order" as "-#order". *)
+    (* iCrash. *)
+    (* iDestruct "pers" as "(persisted & (%CV & % & [% %] & #crash))". *)
+    (* iDestruct (or_lost_get with "crash isNaLoc") as "isNaLoc"; first done. *)
+    (* iDestruct (or_lost_get with "crash order") as "order"; first done. *)
+    (* iDestruct (or_lost_get with "crash knowSV") as "knowSV"; first done. *)
+    (* iDestruct (or_lost_with_t_get with "crash hist") as (s) "(% & ? & ? & _)"; *)
+    (*   first done. *)
+    (* iExists s. *)
+    (* iPureGoal. { by eapply map_slice_no_later_elem_of. } *)
+    (* iSplit. *)
+    (* - iExists 0, 0, ∅, _, (Msg _ ∅ ∅ ∅). iFrame. *)
+    (*   iPureGoal. { apply increasing_list_singleton. } *)
+    (*   iPureGoal. { by rewrite lookup_singleton. } *)
+    (*   iPureGoal. { apply map_no_later_singleton. } *)
+    (*   iPureGoal. { simpl. by rewrite lookup_singleton. } *)
+    (*   iSplit. { admit. } (* FIXME: We'd need to add some post crash rule for this. *) *)
+    (*   iStopProof. *)
+    (*   iStartProof (iProp _). iIntros (?) "_ !%". *)
+    (*   split_and!; try done. *)
+    (*   destruct i as [[??]?]; repeat split; apply view_empty_least. *)
+    (* - iExists _. iFrame "∗#". iPureIntro. apply elem_of_dom. naive_solver. *)
+  (* Admitted. *)
+
+  Lemma monPred_in_bottom : ⊢@{dPropI Σ} monPred_in (∅, ∅, ∅).
+  Proof.
+    iStartProof (iProp _). iPureIntro.
+    intros [[??]?].
+    repeat split; apply view_empty_least.
+  Qed.
+
+  Lemma post_crash_mapsto_na ℓ prot q (ss : list ST) :
+    ℓ ↦_{prot}^{q} ss -∗
+    post_crash (λ hG', or_lost ℓ (∃ s, ⌜s ∈ ss⌝ ∗ ℓ ↦_{prot}^{q} [bumper prot s] ∗
+                                  recovered_at ℓ (bumper prot s))).
+  Proof.
+    rewrite /mapsto_na.
+    iNamed 1.
+    iDestruct "locationProtocol" as "(-#pred & -#order & -#bumper)".
+    iDestruct "isNaLoc" as "-#isNaLoc".
+    iDestruct (post_crash_know_full_history_loc with "[$bumper $hist]") as "H".
+    iDestruct "physMsg" as "-#physMsg".
+    iDestruct "pers" as "-#pers".
+    iCrash.
+    iDestruct "pers" as "#pers".
+    iCombine "knowSV pred order isNaLoc H physMsg" as "H".
+    rewrite /or_lost. rewrite !or_lost_with_t_sep.
+    iApply (or_lost_with_t_mono_strong with "[] H").
+    iIntros (??). iNamed 1.
+    iIntros "(A & B & C & D & E & F)".
+    iDestruct "E" as (sNew ?) "(bump & fullHist & fragHist)".
+    iExists (sNew).
+
+    iAssert (⌜ tP ≤ t ⌝)%I as %?.
+    { iDestruct "pers" as "[(_ & (%CV' & % & [% %] & crashed'))|->]";
+        last (iPureIntro; lia).
+      iDestruct (crashed_at_agree with "crashed crashed'") as %<-.
+      iPureIntro.
+      assert (t = t'); last lia.
+      congruence. }
+    iSplit.
+    { iPureIntro. apply: map_slice_lookup_between; try done.
+      split; first done.
+      eapply map_no_later_Some; naive_solver. }
+    iDestruct "F" as (v) "hist".
+
+    rewrite /recovered_at.
+    iSplit.
+    + iExists 0, 0, ∅, _, (Msg _ ∅ ∅ ∅). iFrame. iFrame "#".
+      iPureGoal. { apply increasing_list_singleton. }
+      iPureGoal. { by rewrite lookup_singleton. }
+      iPureGoal. { apply map_no_later_singleton. }
+      iPureGoal. { by rewrite lookup_singleton. }
+      iSplit. { simpl. iApply monPred_in_bottom. }
+      done.
+    + iExists _. iFrame "∗#".
+      iPureIntro. rewrite elem_of_dom. naive_solver.
+  Qed.
+
+  Global Instance mapsto_na_into_crash `{AbstractState ST} ℓ prot q (ss : list ST) :
+    IntoCrash
+      (ℓ ↦_{prot}^{q} ss)%I
+      (λ hG', or_lost ℓ (∃ s, ⌜s ∈ ss⌝ ∗ ℓ ↦_{prot}^{q} [s] ∗ recovered_at ℓ s))%I.
+  Proof. rewrite /IntoCrash. iIntros "P". by iApply post_crash_mapsto_na. Qed.
+
+  Lemma post_crash_flush_know_flush_lb (ℓ : loc) prot (s : ST) :
+    know_flush_lb ℓ prot s -∗
+    <PCF> hG, ∃ s__pc, ⌜s ⊑ s__pc⌝ ∗
+      recovered_at ℓ s__pc ∗ know_persist_lb ℓ prot s__pc.
+  Proof.
+    iStartProof (iProp _).
+    iIntros (TV).
+    rewrite /know_flush_lb.
+    simpl.
+    iNamed 1.
+    iIntros (???).
+    (*
+    iDestruct (post_crash_modality.post_crash_nodep with "order") as "order".
+    iDestruct (post_crash_modality.post_crash_nodep with "knowFragHist") as "knowFragHist".
+    iDestruct "viewFact" as "[[%neq %leq] | [%eq pers]]".
+    * base.post_crash_modality.iCrash.
+      iNamed 1.
+      rewrite /post_crash_resource.
+      iFrameNamed.
+      iDestruct ("post_crash_history_impl" with "knowFragHist") as "knowFragHist".
+      iDestruct ("post_crash_preorder_impl" with "order") as "order'".
+      iIntros (CV).
+      iIntros (??) "(% & #pers & #crash)".
+      simpl.
+      destruct (flush_view TV !! ℓ) as [[tF']|] eqn:eq; last first.
+      { exfalso.
+        rewrite /lookup_zero in leq.
+        rewrite eq in leq.
+        simpl in leq.
+        lia. }
+      edestruct view_le_look as (t'' & lookCV & lt); [apply eq|eassumption |].
+      iDestruct (or_lost_post_crash_lookup CV with "crash order'") as "#order";
+        first apply lookCV.
+      iDestruct (or_lost_post_crash_lookup CV with "crash knowFragHist")
+        as "(%s'' & %imp & knowFragHist)";
+        first apply lookCV.
+      assert (s ⊑ s'') as sInclS''.
+      { etrans; first done. apply imp.
+        etrans; first done.
+        rewrite /lookup_zero.
+        rewrite eq.
+        simpl. done. }
+      iAssert (persisted_loc ℓ 0) as "persisted".
+      { iApply (persisted_persisted_loc with "pers").
+        rewrite /view_to_zero.
+        rewrite lookup_fmap.
+        rewrite eq.
+        done. }
+      iExists s''.
+      iSplit. { done. }
+      iSplit. { iExists CV. iFrame "crash knowFragHist". iPureIntro.
+                apply elem_of_dom. done. }
+      iSplit. { iExists 0. iFrameNamed. iPureIntro. lia. }
+      iSplit.
+      { iExists 0.
+        iFrameNamed.
+        iRight. by iFrame "#". }
+      iExists 0.
+      iFrameNamed.
+      iPureIntro. apply lookup_zero_gt_zero.
+    * base.post_crash_modality.iCrash.
+      iNamed 1.
+      rewrite /post_crash_resource.
+      iFrameNamed.
+      iDestruct ("post_crash_frag_history_impl" with "knowFragHist") as "knowFragHist".
+      iDestruct ("post_crash_preorder_impl" with "order") as "order'".
+      iIntros (CV).
+      iIntros (??) "(% & #pers' & #crash)".
+      simpl.
+      iDestruct "pers" as "[#persisted (%CV' & %t & [%lookCV _] & crash')]".
+      iDestruct (crashed_at_agree with "crash crash'") as %<-.
+      iClear "crash'".
+      iDestruct (or_lost_post_crash_lookup CV with "crash order'") as "#order";
+        first apply lookCV.
+      iDestruct (or_lost_post_crash_lookup CV with "crash knowFragHist")
+        as "(%s'' & %imp & knowFragHist)";
+        first apply lookCV.
+      assert (s ⊑ s'') as sInclS''.
+      { etrans; first done. apply imp.
+        etrans; first done.
+        rewrite /lookup_zero.
+        rewrite eq.
+        lia. }
+      iExists s''.
+      iSplit. { done. }
+      iSplit. { iExists CV. iFrame "crash knowFragHist". iPureIntro.
+                apply elem_of_dom. done. }
+      iSplit.
+      { iExists 0. iFrameNamed. iPureIntro. lia. }
+      iSplit.
+      { iExists 0. iFrameNamed. iRight. by iFrame "#". }
+      iExists 0. iFrameNamed. iPureIntro. lia.
+     *)
+  Admitted.
+
+  Global Instance know_flush_into_crash ℓ prot (s : ST) :
+    IntoCrashFlush (know_flush_lb ℓ prot s) (λ _, ∃ s__pc, ⌜ s ⊑ s__pc ⌝ ∗
+      recovered_at ℓ s__pc ∗ know_persist_lb ℓ prot s__pc)%I.
+  Proof.
+    rewrite /IntoCrashFlush. iIntros "P".
+    by iApply post_crash_flush_know_flush_lb.
+  Qed.
+  (* Global Instance mapsto_na_persisted_into_crash `{AbstractState ST} ℓ (ss : list ST) : *)
+  (*   IntoCrash (ℓ ↦_{true} ss)%I (λ hG', ∃ s, ⌜s ∈ ss⌝ ∗ ℓ ↦_{true} [s] ∗ recovered_at ℓ s)%I. *)
+  (* Proof. *)
+  (*   rewrite /IntoCrash. iIntros "P". by iApply post_crash_mapsto_persisted_ex. *)
+  (* Qed. *)
+
+  Lemma recovered_at_or_lost `{AbstractState ST} ℓ P (s : ST) :
+    recovered_at ℓ s -∗ or_lost ℓ P -∗ P.
+  Proof.
+    iNamed 1. iIntros "P".
+    iApply (or_lost_get with "crashed P").
+    apply elem_of_dom.
+    done.
+  Qed.
+
+End points_to_at_more.
+
+Typeclasses Opaque mapsto_na.
+Typeclasses Opaque know_store_lb.
+Typeclasses Opaque know_flush_lb.
+Typeclasses Opaque know_persist_lb.
